

Úloha 1

$$a = [1, 1, 1]^T$$

$$x = [x_1, x_2, x_3]^T$$

$$B = \begin{bmatrix} 1 & -2 & 3 \\ -2 & 3 & 3 \\ 3 & 3 & 2 \end{bmatrix}$$

a. $a^T x$

$$a^T x = [1 \quad 1 \quad 1] \begin{bmatrix} x_1 \\ x_2 \\ x_3 \end{bmatrix} = x_1 + x_2 + x_3$$

b. ax^T

$$ax^T = \begin{bmatrix} 1 \\ 1 \\ 1 \end{bmatrix} [x_1 \quad x_2 \quad x_3] = \begin{bmatrix} x_1 & x_2 & x_3 \\ x_1 & x_2 & x_3 \\ x_1 & x_2 & x_3 \end{bmatrix}$$

c. Ba

$$Ba = \begin{bmatrix} 1 & -2 & 3 \\ -2 & 3 & 3 \\ 3 & 3 & 2 \end{bmatrix} \begin{bmatrix} 1 \\ 1 \\ 1 \end{bmatrix} = \begin{bmatrix} 2 \\ 4 \\ 8 \end{bmatrix}$$

d. $\frac{\partial x^T B x}{\partial x}$

$$x^T B x = [x_1 \quad x_2 \quad x_3] \begin{bmatrix} 1 & -2 & 3 \\ -2 & 3 & 3 \\ 3 & 3 & 2 \end{bmatrix} \begin{bmatrix} x_1 \\ x_2 \\ x_3 \end{bmatrix}$$

$$x^T B = [x_1 \quad x_2 \quad x_3] \begin{bmatrix} 1 & -2 & 3 \\ -2 & 3 & 3 \\ 3 & 3 & 2 \end{bmatrix} = [x_1 - 2x_2 + 3x_3 \quad -2x_1 + 3x_2 + 3x_3 \quad 3x_1 + 3x_2 + 2x_3]$$

$$x^T B x = (x_1 - 2x_2 + 3x_3)x_1 + (-2x_1 + 3x_2 + 3x_3)x_2 + (3x_1 + 3x_2 + 2x_3)x_3 = x_1^2 - 2x_1x_2 + 3x_1x_3 +$$

$$x^T Bx = x_1^2 - 4x_1x_2 + 6x_1x_3 + 3x_2^2 + 6x_2x_3 + 2x_3^2$$

$$\frac{\partial}{\partial x_1}(x^T Bx) = 2x_1 - 4x_2 + 6x_3$$

$$\frac{\partial}{\partial x_2}(x^T Bx) = -4x_1 + 6x_2 + 6x_3$$

$$\frac{\partial}{\partial x_3}(x^T Bx) = 6x_1 + 6x_2 + 4x_3$$

$$\frac{\partial x^T Bx}{\partial x} = \begin{bmatrix} 2x_1 - 4x_2 + 6x_3 \\ -4x_1 + 6x_2 + 6x_3 \\ 6x_1 + 6x_2 + 4x_3 \end{bmatrix}$$